define well-formed config/state and prove properties
introduce `wf_state` for current state and symbols under TM-head
introduce `wf_config` for current state and contents of all tapes
change wf_TM locale axioms to require `wf_state` consistently
prove `final_step_fixpoint` (after adding `wf_state` as assumption)
prove `wf_config_step` (performing a `step` on a `wf_state` results in another `wf_state`)
prove that the `start_config` is well-formed, and thus `run n w` is as well (if `w` only contains allowed symbols)

papers/116_stefan_rass/TM.thy
@@ -6,8 +6,8 @@ class blank =
   fixes Bk :: 'a
 
 instantiation nat :: blank begin
-  definition Bk_nat :: nat where "Bk_nat = 0"
-  instance ..
+definition Bk_nat :: nat where "Bk_nat = 0"
+instance ..
 end
 
 datatype 'b action = L | R | W 'b | Nop
@@ -15,30 +15,65 @@ datatype 'b action = L | R | W 'b | Nop
 fun symbol_of_write :: "'b action \<Rightarrow> 'b::blank" where
   "symbol_of_write (W w) = w" | "symbol_of_write _ = Bk"
 
+lemma symbol_of_write_def: "symbol_of_write a = (case a of W w \<Rightarrow> w | _ \<Rightarrow> Bk)"
+  by (induction a) auto
+
+
 record 'b tape =
   left :: "'b list"
   right :: "'b list"
 
 abbreviation "empty_tape \<equiv> \<lparr>left=[], right=[]\<rparr>"
 
+definition [simp]: "set_of_tape tp \<equiv> set (left tp) \<union> set (right tp) \<union> {Bk}"
+
+
 text\<open>TM execution begins with the head at the start of the input word.\<close>
 abbreviation input_tape ("<_>\<^sub>t\<^sub>p") where "<w>\<^sub>t\<^sub>p \<equiv> \<lparr>left=[], right=w\<rparr>"
 
-abbreviation size :: "'b tape \<Rightarrow> nat" where
-  "size tp \<equiv> length (left tp) + length (right tp)"
+abbreviation tp_size :: "'b tape \<Rightarrow> nat" where
+  "tp_size tp \<equiv> length (left tp) + length (right tp)"
 
 fun tp_update :: "('b::blank) action \<Rightarrow> 'b tape \<Rightarrow> 'b tape" where
- "tp_update  L     \<lparr>left=[]  , right=rs  \<rparr> = \<lparr>left=[]   , right=Bk#rs\<rparr>"
-|"tp_update  L     \<lparr>left=l#ls, right=rs  \<rparr> = \<lparr>left=ls   , right=l#rs \<rparr>"
-|"tp_update  R     \<lparr>left=ls  , right=[]  \<rparr> = \<lparr>left=Bk#ls, right=[]   \<rparr>"
-|"tp_update  R     \<lparr>left=ls  , right=r#rs\<rparr> = \<lparr>left=r#ls , right=rs   \<rparr>"
-|"tp_update (W w)  \<lparr>left=ls  , right=[]  \<rparr> = \<lparr>left=ls   , right=[w]  \<rparr>"
-|"tp_update (W w)  \<lparr>left=ls  , right=r#rs\<rparr> = \<lparr>left=ls   , right=w#rs \<rparr>"
-|"tp_update Nop tape = tape"
+  "tp_update  L     \<lparr>left=[]  , right=rs  \<rparr> = \<lparr>left=[]   , right=Bk#rs\<rparr>"
+| "tp_update  L     \<lparr>left=l#ls, right=rs  \<rparr> = \<lparr>left=ls   , right=l#rs \<rparr>"
+| "tp_update  R     \<lparr>left=ls  , right=[]  \<rparr> = \<lparr>left=Bk#ls, right=[]   \<rparr>"
+| "tp_update  R     \<lparr>left=ls  , right=r#rs\<rparr> = \<lparr>left=r#ls , right=rs   \<rparr>"
+| "tp_update (W w)  \<lparr>left=ls  , right=[]  \<rparr> = \<lparr>left=ls   , right=[w]  \<rparr>"
+| "tp_update (W w)  \<lparr>left=ls  , right=r#rs\<rparr> = \<lparr>left=ls   , right=w#rs \<rparr>"
+| "tp_update Nop tape = tape"
+
+
+lemma tp_update_set: "set_of_tape (tp_update a tp) \<subseteq> set_of_tape tp \<union> {symbol_of_write a}"
+proof -
+  obtain l r where expand_tp: "tp = \<lparr>left=l,right=r\<rparr>" by (rule tape.cases)
+  show ?thesis unfolding expand_tp
+  proof (induction a)
+    case L thus ?case by (induction l) auto next
+    case R thus ?case by (induction r) auto next
+    case (W x) thus ?case by (induction r) auto next
+    case Nop thus ?case by simp
+  qed
+qed
+
 
 fun tp_read :: "('b :: blank) tape \<Rightarrow> 'b" where
   "tp_read \<lparr>left=_, right=[]  \<rparr> = Bk"
 | "tp_read \<lparr>left=_, right=r#rs\<rparr> = r"
+
+lemma tp_read_def: "tp_read tp = (if right tp = [] then Bk else hd (right tp))"
+proof (cases "right tp")
+  case Nil
+  then have expand_tp: "tp = \<lparr> left=left tp, right = [] \<rparr>" by simp
+  from \<open>right tp = []\<close> show ?thesis by (subst expand_tp) simp
+next
+  case (Cons t ts)
+  then have expand_tp: "tp = \<lparr> left=left tp, right = t#ts \<rparr>" by simp
+  from \<open>right tp = t # ts\<close> show ?thesis by (subst expand_tp) simp
+qed
+
+corollary tp_read_symbol: "tp_read tp \<in> set (right tp) \<union> {Bk}" unfolding tp_read_def by simp
+
 
 record ('a, 'b) TM =
   tape_count :: nat
@@ -49,29 +84,98 @@ record ('a, 'b) TM =
   accepting_states :: "'a set"
 
   symbols :: "'b set"
-    
+
   next_state  :: "'a \<Rightarrow> 'b list \<Rightarrow> 'a"
   next_action :: "'a \<Rightarrow> 'b list \<Rightarrow> 'b action list"
 
 record ('a, 'b) TM_config =
   state :: 'a
-  tapes  :: "'b tape list"
+  tapes :: "'b tape list"
+
+
+\<comment> \<open>A state \<open>q\<close> in combination with a vector (\<^typ>\<open>'b list\<close>) of symbols currently under the TM-heads \<open>w\<close>,
+  is considered a well-formed state w.r.t. a \<^typ>\<open>('a, 'b) TM\<close> \<open>M\<close>, iff
+  \<open>q\<close> is a valid state for \<open>M\<close>,
+  the number of elements of \<open>w\<close> matches the number of tapes of \<open>M\<close>, and
+  all elements of \<open>w\<close> are valid symbols for \<open>M\<close> (members of \<open>M\<close>'s tape alphabet).\<close>
+definition wf_state_wrt_TM :: "('a, 'b) TM \<Rightarrow> 'a \<Rightarrow> 'b list \<Rightarrow> bool" where
+  "wf_state_wrt_TM M q w \<equiv> q \<in> states M \<and> length w = tape_count M \<and> set w \<subseteq> symbols M"
+
+lemma wf_stateI[intro]:
+  "\<lbrakk>q\<in>states M; length w = tape_count M; set w \<subseteq> symbols M\<rbrakk> \<Longrightarrow> wf_state_wrt_TM M q w"
+  unfolding wf_state_wrt_TM_def by blast
+lemma wf_stateE[elim]:
+  assumes "wf_state_wrt_TM M q w" shows "q \<in> states M" "length w = tape_count M" "set w \<subseteq> symbols M"
+  using assms unfolding wf_state_wrt_TM_def by blast+
+
+\<comment> \<open>A \<^typ>\<open>('a, 'b) TM_config\<close> \<open>c\<close> is considered well-formed w.r.t. a \<^typ>\<open>('a, 'b) TM\<close> \<open>M\<close>, iff
+  the \<^const>\<open>state\<close> of \<open>c\<close> is valid for \<open>M\<close>,
+  the number of \<^const>\<open>tapes\<close> of \<open>c\<close> matches the number of tapes of \<open>M\<close>, and
+  all symbols on all \<^const>\<open>tapes\<close> of \<open>c\<close> are valid symbols for \<open>M\<close>.\<close>
+definition wf_config_wrt_TM :: "('a, 'b :: blank) TM \<Rightarrow> ('a, 'b) TM_config \<Rightarrow> bool" where
+  "wf_config_wrt_TM M c \<equiv> let q = state c; ts = tapes c in
+        q \<in> states M
+      \<and> length ts = tape_count M
+      \<and> \<Union> (set_of_tape ` set ts) \<subseteq> symbols M"
+
+lemma wf_configI[intro]:
+  assumes "state c \<in> states M"
+    and "length (tapes c) = tape_count M"
+    and "\<Union> (set_of_tape ` set (tapes c)) \<subseteq> symbols M"
+  shows "wf_config_wrt_TM M c"
+  unfolding wf_config_wrt_TM_def Let_def using assms by blast
+lemma wf_configE[elim]:
+  assumes "wf_config_wrt_TM M c"
+  shows "state c \<in> states M"
+    and "length (tapes c) = tape_count M"
+    and "\<Union> (set_of_tape ` set (tapes c)) \<subseteq> symbols M"
+  using assms unfolding wf_config_wrt_TM_def Let_def by blast+
+
 
 locale wf_TM =
   fixes M :: "('a, 'b::blank) TM" (structure)
-  assumes "1 \<le> tape_count M"
-  and "finite (states M)" "start_state M \<in> states M" "final_states M \<subseteq> states M"
-  and "accepting_states M \<subseteq> final_states M"
-  and "finite (symbols M)" "Bk \<in> (symbols M)"
-  and "\<forall>q\<in>states M. \<forall>w. length w = tape_count M \<longrightarrow> set w \<subseteq> symbols M \<longrightarrow>
-       next_state M q w \<in> states M
-     \<and> length (next_action M q w) = tape_count M
-     \<and> symbol_of_write ` set (next_action M q w) \<subseteq> symbols M"
-  and final_state: "\<forall>q\<in>final_states M. \<forall>w. next_state M q w = q"
-  and final_action: "\<forall>q\<in>final_states M. \<forall>w. set (next_action M q w) \<subseteq> {Nop}"
+  assumes at_least_one_tape: "1 \<le> tape_count M"
+  and state_axioms: "finite (states M)" "start_state M \<in> states M"
+                    "final_states M \<subseteq> states M" "accepting_states M \<subseteq> final_states M"
+  and symbols_axioms: "finite (symbols M)" "Bk \<in> (symbols M)"
+  and next_state: "\<And>q w. wf_state_wrt_TM M q w \<Longrightarrow> next_state M q w \<in> states M"
+  and next_action_length: "\<And>q w. wf_state_wrt_TM M q w \<Longrightarrow>
+        length (next_action M q w) = tape_count M"
+  and next_write_symbol: "\<And>q w. wf_state_wrt_TM M q w \<Longrightarrow>
+        symbol_of_write ` set (next_action M q w) \<subseteq> symbols M"
+  and final_state: "\<And>q w. wf_state_wrt_TM M q w \<Longrightarrow> q \<in> final_states M \<Longrightarrow>
+        next_state M q w = q"
+  and final_action: "\<And>q w. wf_state_wrt_TM M q w \<Longrightarrow> q \<in> final_states M \<Longrightarrow>
+        set (next_action M q w) \<subseteq> {Nop}"
 begin
-definition is_final :: "('a, 'b) TM_config \<Rightarrow> bool" where
-  "is_final c \<longleftrightarrow> state c \<in> final_states M"
+
+abbreviation wf_state where "wf_state \<equiv> wf_state_wrt_TM M"
+abbreviation wf_config where "wf_config \<equiv> wf_config_wrt_TM M"
+
+abbreviation wf_state_of_config ("wf'_state\<^sub>c")
+  where "wf_state\<^sub>c c \<equiv> wf_state (state c) (map tp_read (tapes c))"
+
+lemma wf_config_state: "wf_config c \<Longrightarrow> wf_state\<^sub>c c"
+proof
+  let ?q = "state c" and ?ts = "tapes c"
+  assume "wf_config c"
+  then show "?q \<in> states M" ..
+
+  from \<open>wf_config c\<close> have "length ?ts = tape_count M" ..
+  then show "length (map tp_read (tapes c)) = tape_count M" by simp
+
+  have "set (map tp_read ?ts) \<subseteq> \<Union> (set_of_tape ` set (tapes c))"
+    unfolding set_map set_of_tape_def using tp_read_symbol by blast
+  also have "... \<subseteq> symbols M" using \<open>wf_config c\<close> ..
+  finally show "set (map tp_read (tapes c)) \<subseteq> symbols M" .
+qed
+
+corollary wf_state_tape_count: "wf_state\<^sub>c c \<Longrightarrow> length (tapes c) = tape_count M"
+  unfolding wf_state_wrt_TM_def by simp
+
+
+abbreviation is_final :: "('a, 'b) TM_config \<Rightarrow> bool" where
+  "is_final c \<equiv> state c \<in> final_states M"
 
 definition step :: "('a, 'b) TM_config \<Rightarrow> ('a, 'b) TM_config" where
   "step c = (let q=state c; w=map tp_read (tapes c) in \<lparr>
@@ -79,13 +183,86 @@ definition step :: "('a, 'b) TM_config \<Rightarrow> ('a, 'b) TM_config" where
       tapes=map2 tp_update (next_action M q w) (tapes c)
    \<rparr>)"
 
-lemma final_step_fixpoint: "is_final c \<Longrightarrow> step c = c"
-  sorry
+abbreviation all_Nop ("Nop\<^sub>k") where "Nop\<^sub>k \<equiv> replicate (tape_count M) Nop"
 
-lemma final_steps: "\<And>n. is_final c \<Longrightarrow> (step^^n) c = c"
-  using final_step_fixpoint[of c] funpow_fixpoint by metis
 
-definition start_config :: "'b list \<Rightarrow> ('a, 'b) TM_config" where
+corollary all_Nop_update[simp]: "length ts = tape_count M \<Longrightarrow> map2 tp_update Nop\<^sub>k ts = ts"
+  unfolding map2_replicate by (simp add: map_idI)
+
+lemma final_action_explicit:
+  "\<lbrakk>wf_state q w; q \<in> final_states M\<rbrakk> \<Longrightarrow> next_action M q w = Nop\<^sub>k"
+  using next_action_length final_action by (intro replicate_eqI) blast+
+
+lemma final_step_fixpoint:
+  assumes wf: "wf_state\<^sub>c c" and fc: "is_final c"
+  shows "step c = c"
+proof -
+  let ?q = "state c" and ?w = "map tp_read (tapes c)" and ?ts = "tapes c"
+
+  have ns: "next_state M ?q ?w = ?q" using wf fc by (rule final_state)
+  have na: "next_action M ?q ?w = Nop\<^sub>k" using wf fc by (rule final_action_explicit)
+  have tu: "map2 tp_update Nop\<^sub>k ?ts = ?ts" using all_Nop_update wf_state_tape_count wf .
+
+  show "step c = c" unfolding step_def Let_def unfolding ns na tu by simp
+qed
+
+lemma final_steps: "wf_state\<^sub>c c \<Longrightarrow> is_final c \<Longrightarrow> (step^^n) c = c"
+  by (intro funpow_fixpoint) (rule final_step_fixpoint)
+
+
+lemma nth_map2:
+  assumes "i < length xs" and "i < length ys"
+  shows "map2 f xs ys ! i = f (xs ! i) (ys ! i)"
+  using assms by (subst nth_map) auto
+
+lemma wf_config_step: "wf_config c \<Longrightarrow> wf_config (step c)"
+proof
+  let ?q = "state c" and ?w = "map tp_read (tapes c)" and ?ts = "tapes c"
+  let ?q' = "state (step c)" and ?ts' = "tapes (step c)"
+  let ?na = "next_action M ?q ?w"
+  assume "wf_config c"
+  then have wf: "wf_state\<^sub>c c" by (rule wf_config_state)
+
+  from \<open>wf_config c\<close> have "?q \<in> states M" ..
+  have q': "?q' = next_state M ?q ?w" unfolding step_def Let_def by simp
+  show "?q' \<in> states M" unfolding q' using wf by (rule next_state)
+
+  have lna: "length ?na = tape_count M" using wf by (rule next_action_length)
+  moreover have lts: "length ?ts = tape_count M" using \<open>wf_config c\<close> ..
+  ultimately show lts': "length ?ts' = tape_count M" unfolding step_def Let_def by simp
+
+  have "\<forall>i < length ?ts'. set_of_tape (?ts' ! i) \<subseteq> symbols M" unfolding lts'
+  proof (intro allI impI)
+    fix i assume "i < tape_count M"
+    have *: "?ts' ! i = tp_update (?na ! i) (?ts ! i)" unfolding step_def Let_def TM_config.simps(2)
+      using lna lts \<open>i < tape_count M\<close> by (intro nth_map2) auto
+
+    have "set_of_tape (?ts' ! i) \<subseteq> set_of_tape (?ts ! i) \<union> {symbol_of_write (?na ! i)}"
+      unfolding * by (rule tp_update_set)
+    also have "... \<subseteq> symbols M"
+    proof (intro Un_least)
+      have "i < length ?ts" unfolding lts by (fact \<open>i < tape_count M\<close>)
+      from \<open>wf_config c\<close> have "\<Union> (set_of_tape ` set ?ts) \<subseteq> symbols M" ..
+      then have "\<forall>tp \<in> set ?ts. set_of_tape tp \<subseteq> symbols M" by blast
+      with \<open>i < length ?ts\<close> show "set_of_tape (?ts ! i) \<subseteq> symbols M" by (rule list_ball_nth)
+
+      have "i < length ?na" unfolding lna by (fact \<open>i < tape_count M\<close>)
+      from \<open>wf_state\<^sub>c c\<close> have "symbol_of_write ` set ?na \<subseteq> symbols M" by (rule next_write_symbol)
+      then have "\<forall>tp \<in> set ?na. symbol_of_write tp \<in> symbols M" by blast
+      with \<open>i < length ?na\<close> show "{symbol_of_write (?na ! i)} \<subseteq> symbols M"
+        by (intro list_ball_nth) blast+
+    qed
+    finally show "set_of_tape (?ts' ! i) \<subseteq> symbols M" .
+  qed
+  then have "\<forall>tp \<in> set ?ts'. set_of_tape tp \<subseteq> symbols M" unfolding all_set_conv_all_nth .
+  then show "\<Union> (set_of_tape ` set ?ts') \<subseteq> symbols M" by blast
+qed
+
+corollary wf_config_steps: "wf_config c \<Longrightarrow> wf_config ((step^^n) c)"
+  using wf_config_step by (induction n) auto
+
+
+definition start_config :: "'b list \<Rightarrow> ('a, 'b) TM_config" where [simp]:
   "start_config w = \<lparr>
     state = start_state M,
     tapes = <w>\<^sub>t\<^sub>p # replicate (tape_count M - 1) empty_tape
@@ -93,17 +270,37 @@ definition start_config :: "'b list \<Rightarrow> ('a, 'b) TM_config" where
 
 abbreviation "run n w \<equiv> (step^^n) (start_config w)"
 
+
+lemma wf_start_config: "set w \<subseteq> symbols M \<Longrightarrow> wf_config (start_config w)"
+proof
+  show "state (start_config w) \<in> states M" using state_axioms(2) by simp
+  show "length (tapes (start_config w)) = tape_count M" using at_least_one_tape by simp
+
+  assume "set w \<subseteq> symbols M"
+  have "set (tapes (start_config w)) \<subseteq> {<w>\<^sub>t\<^sub>p, empty_tape}" by fastforce
+  moreover have "set_of_tape empty_tape = {Bk}" by simp
+  moreover have "set_of_tape <w>\<^sub>t\<^sub>p = set w \<union> {Bk}" by simp
+  ultimately have "\<Union> (set_of_tape ` set (tapes (start_config w))) \<subseteq> set w \<union> {Bk}" by blast
+  also have "... \<subseteq> symbols M" using \<open>set w \<subseteq> symbols M\<close> symbols_axioms(2) by blast
+  finally show "\<Union> (set_of_tape ` set (tapes (start_config w))) \<subseteq> symbols M" .
+qed
+
+corollary wf_config_run: "set w \<subseteq> symbols M \<Longrightarrow> wf_config (run n w)"
+  using wf_start_config by (rule wf_config_steps)
+
+
 lemma final_le_steps:
-  assumes "is_final ((step^^n) c)"
+  assumes "wf_config c"
+      and "is_final ((step^^n) c)"
       and "n \<le> m"
     shows "(step^^m) c = (step^^n) c"
 proof -
-  from \<open>n\<le>m\<close> obtain n' where "m = n' + n"
-    by (metis add.commute less_eqE)
-  then have "(step^^m) c = (step^^n') ((step^^n) c)"
-    using funpow_add[of n' n step] by simp
-  thus "(step^^m) c = (step^^n) c"
-    using final_steps[of "(step^^n) c" n'] assms(1) by simp
+  from \<open>n\<le>m\<close> obtain n' where "m = n' + n" by (metis add.commute less_eqE)
+  have wf: "wf_state\<^sub>c ((step^^n) c)" using wf_config_state wf_config_steps \<open>wf_config c\<close> .
+  have "(step^^m) c = (step^^n') ((step^^n) c)"
+    unfolding \<open>m = n' + n\<close> funpow_add by (rule comp_apply)
+  also have "... = (step^^n) c" using wf assms(2) by (rule final_steps)
+  finally show "(step^^m) c = (step^^n) c" .
 qed
 
 end \<comment> \<open>\<^locale>\<open>wf_TM\<close>\<close>
@@ -124,7 +321,7 @@ fun tm_comp :: "('a1, 'b::blank) TM \<Rightarrow> ('a2, 'b) TM \<Rightarrow> ('a
     final_states = Inr`final_states M2,
     accepting_states = Inr`accepting_states M2,
     symbols = symbols M1 \<union> symbols M2,
-    next_state = (\<lambda>q w. case q of 
+    next_state = (\<lambda>q w. case q of
                         Inl q1 \<Rightarrow> let w1 = nths w {0..<tape_count M1} in
                                   let q' = next_state M1 q1 w1 in
                                   if q' \<in> final_states M1
@@ -144,6 +341,7 @@ fun tm_comp :: "('a1, 'b::blank) TM \<Rightarrow> ('a2, 'b) TM \<Rightarrow> ('a
 
 lemma "wf_TM M1 \<Longrightarrow> wf_TM M2 \<Longrightarrow> wf_TM (M1 |+| M2)"
   sorry
+
 
 subsection \<open>Hoare Rules\<close>
 
